Execution_resources/grids.v
@@ -3,9 +3,9 @@ From Views Require Import utils.
 From Views.Execution_resources Require Import Execution_resources.
 From Views.Execution_resources Require Import lemmas.
 From Views.Execution_resources Require Import blocks.
+From Views.Execution_resources Require Import correctness_lemmas.
 From Views.Execution_resources Require Import sets_of_threads.
 Require Import PeanoNat.
-
 
 Proposition grid_not_contain_larger_on_z :
   forall z x y x' y' z' idx idy idz i j k,
@@ -796,6 +796,159 @@ Proof.
   apply grid_contain_smaller_on_xyz.
 Qed.
 
+
+Proposition blocks_correct :
+  forall i e m,
+  no_error e blocks -> count i (thread_set' e) m -> count i (thread_set' (blocks e)) m
+.
+Proof.
+  induction e; intros; try (exfalso; apply H; reflexivity).
+  - destruct shp as [[x y] z], shp' as [[x' y'] z']. simpl in *.
+    rewrite grid_ok_xyz in H0. apply H0.
+  - simpl in *. assert (forall i n v n0,
+          (forall n' n0, n' < n ->
+                count i (thread_set' (v n')) n0 ->
+                count i (thread_set' (blocks (v n'))) n0) ->
+            count i (zip (buildList n (fun i : nat => thread_set' (v i)))) n0 ->
+            count i (zip (buildList n (fun i0 : nat => thread_set' (blocks (v i0))))) n0). {
+        clear.
+        induction n.
+        + intros. apply H0.
+        + intros. simpl in *.
+        apply cat_count_rev in H0.
+        destruct H0 as [m [m' [H0 [H1 H2]]]]. subst.
+        apply cat_count.
+        apply H. apply le_n. apply H0.
+        apply IHn. intros. apply le_S in H2. apply H with (n0 := n0) in H2. apply H2. apply H3.
+        apply H1.
+    }
+    apply H2. intros.
+    apply H with (n := n') (m := n0) in H0.
+    apply H0. apply H3. apply H4. apply H1.
+  - simpl in *. assert (forall a x y z v n,
+          (forall i j k n, i < x -> j < y -> k < z ->
+                count a (thread_set' (v i j k)) n ->
+                count a (thread_set' (blocks (v i j k))) n) ->
+            count a (thread_set' (TensorCollection x y z v)) n ->
+            count a (thread_set' (blocks (TensorCollection x y z v))) n). {
+        clear.
+        induction x.
+        + intros. apply H0.
+        + intros. simpl in *.
+          apply cat_count_rev in H0.
+          destruct H0 as [m [m' [H0 [H1 H2]]]]. subst.
+          apply cat_count. clear H1. clear IHx.
+          generalize dependent m. induction y.
+          - intros. apply H0.
+          - intros. simpl in *. apply cat_count_rev in H0.
+            destruct H0 as [m0 [m0' [H0 [H1 H2]]]]. subst.
+            apply cat_count. clear H1. clear IHy.
+            generalize dependent m0. induction z.
+            * intros. apply H0.
+            * intros. simpl in *. apply cat_count_rev in H0.
+              destruct H0 as [m1 [m1' [H0 [H1 H2]]]]. subst.
+              apply cat_count. apply H. apply le_n. apply le_n. apply le_n.
+              apply H0. apply IHz. intros. apply H.
+              apply H2. apply H3. apply le_S in H4. apply H4. apply H5.
+              apply H1.
+          * apply IHy. intros. apply H.
+          apply H2. apply le_S in H3. apply H3. apply H4. apply H5.
+          apply H1.
+        - apply IHx. intros. apply H.
+        apply le_S in H2. apply H2. apply H3. apply H4. apply H5.
+        apply H1.
+    }
+    apply H2. intros.
+    apply (H i0 j k) with (m := n) in H0.
+    apply H0. apply H3. apply H4. apply H5. apply H6. apply H1.
+Qed.
+
+
+Proposition blocks_correct_physical :
+  forall i e m f,
+  no_error e blocks -> count i (physical_thread_set e f) m -> count i (physical_thread_set (blocks e) f) m
+.
+Proof.
+  induction e; intros; try (exfalso; apply H; reflexivity).
+  - destruct shp as [[x y] z], shp' as [[x' y'] z']. simpl in *.
+    rewrite grid_ok_xyz in H0.
+    clear H. generalize dependent m. induction x.
+    + intros. apply H0.
+    + intros. simpl in *.
+      rewrite map_cat in H0. apply cat_count_rev in H0.
+      destruct H0 as [m0 [m0' [H0 [H1 H2]]]]. subst.
+      apply cat_count. clear H1. clear IHx.
+      generalize dependent m0. induction y.
+      * intros. apply H0.
+      * intros. simpl in *.
+        rewrite map_cat in H0. apply cat_count_rev in H0.
+        destruct H0 as [m1 [m1' [H0 [H1 H2]]]]. subst.
+        apply cat_count. clear H1. clear IHy.
+        generalize dependent m1. induction z.
+        --  intros. apply H0.
+        --  intros. simpl in *.
+            rewrite map_cat in H0. apply cat_count_rev in H0.
+            destruct H0 as [m2 [m2' [H0 [H1 H2]]]]. subst.
+            apply cat_count. apply H0. apply IHz. apply H1.
+      -- apply IHy. apply H1.
+    * apply IHx. apply H1.
+  - simpl in *. assert (forall i n v n0,
+          (forall n' n0, n' < n ->
+                count i (physical_thread_set (v n') f) n0 ->
+                count i (physical_thread_set (blocks (v n')) f) n0) ->
+            count i (zip (buildList n (fun i : nat => physical_thread_set (v i) f))) n0 ->
+            count i (zip (buildList n (fun i0 : nat => physical_thread_set (blocks (v i0)) f))) n0). {
+        clear.
+        induction n.
+        + intros. apply H0.
+        + intros. simpl in *.
+        apply cat_count_rev in H0.
+        destruct H0 as [m [m' [H0 [H1 H2]]]]. subst.
+        apply cat_count.
+        apply H. apply le_n. apply H0.
+        apply IHn. intros. apply le_S in H2. apply H with (n0 := n0) in H2. apply H2. apply H3.
+        apply H1.
+    }
+    apply H2. intros.
+    apply H with (n := n') (m := n0) (f := f) in H0.
+    apply H0. apply H3. apply H4. apply H1.
+  - simpl in *. assert (forall a x y z v n,
+          (forall i j k n, i < x -> j < y -> k < z ->
+                count a (physical_thread_set (v i j k) f) n ->
+                count a (physical_thread_set (blocks (v i j k)) f) n) ->
+            count a (physical_thread_set (TensorCollection x y z v) f) n ->
+            count a (physical_thread_set (blocks (TensorCollection x y z v)) f) n). {
+        clear.
+        induction x.
+        + intros. apply H0.
+        + intros. simpl in *.
+          apply cat_count_rev in H0.
+          destruct H0 as [m [m' [H0 [H1 H2]]]]. subst.
+          apply cat_count. clear H1. clear IHx.
+          generalize dependent m. induction y.
+          - intros. apply H0.
+          - intros. simpl in *. apply cat_count_rev in H0.
+            destruct H0 as [m0 [m0' [H0 [H1 H2]]]]. subst.
+            apply cat_count. clear H1. clear IHy.
+            generalize dependent m0. induction z.
+            * intros. apply H0.
+            * intros. simpl in *. apply cat_count_rev in H0.
+              destruct H0 as [m1 [m1' [H0 [H1 H2]]]]. subst.
+              apply cat_count. apply H. apply le_n. apply le_n. apply le_n.
+              apply H0. apply IHz. intros. apply H.
+              apply H2. apply H3. apply le_S in H4. apply H4. apply H5.
+              apply H1.
+          * apply IHy. intros. apply H.
+          apply H2. apply le_S in H3. apply H3. apply H4. apply H5.
+          apply H1.
+        - apply IHx. intros. apply H.
+        apply le_S in H2. apply H2. apply H3. apply H4. apply H5.
+        apply H1.
+    }
+    apply H2. intros.
+    apply (H i0 j k) with (m := n) (f := f) in H0.
+    apply H0. apply H3. apply H4. apply H5. apply H6. apply H1.
+Qed.
 
 
 
